src/QueryStructure/Implementation/Operations/BagADT/Refinements.v
@@ -1,4 +1,4 @@
- Require Export Coq.Lists.List Coq.Program.Program
+Require Export Coq.Lists.List Coq.Program.Program
         ADTSynthesis.QueryStructure.Specification.Representation.Tuple
         ADTSynthesis.QueryStructure.Specification.Representation.Heading
         ADTSynthesis.Common.ilist
@@ -24,7 +24,7 @@ Section BagsQueryStructureRefinements.
   Variable qs_schema : QueryStructureSchema.
   Variable BagIndexKeys :
     ilist (fun ns => SearchUpdateTerms (schemaHeading (relSchema ns)))
-      (qschemaSchemas qs_schema).
+          (qschemaSchemas qs_schema).
 
   Lemma i2th_Bounded_Initialize_IndexedQueryStructure
   : forall ns indices v idx,
@@ -52,7 +52,7 @@ Section BagsQueryStructureRefinements.
     unfold GetUnConstrRelation.
     unfold DropQSConstraints, QSEmptySpec; split.
     intros; rewrite <- ith_Bounded_imap, ith_Bounded_BuildEmptyRelations,
-    i2th_Bounded_Initialize_IndexedQueryStructure; eauto.
+            i2th_Bounded_Initialize_IndexedQueryStructure; eauto.
     intros; eexists [];
     apply EnsembleIndexedListEquivalence_Empty.
   Qed.
@@ -74,91 +74,10 @@ Section BagsQueryStructureRefinements.
     forall (r_n : IndexedQueryStructure qs_schema BagIndexKeys) idx idx' newRel,
       idx <> idx'
       -> GetIndexedRelation (UpdateIndexedRelation r_n idx newRel) idx' =
-      GetIndexedRelation r_n idx'.
+         GetIndexedRelation r_n idx'.
   Proof.
     unfold UpdateIndexedRelation, GetIndexedRelation;
     intros; simpl; rewrite i2th_replace_BoundIndex_neq; eauto using string_dec.
-  Qed.
-
-  (* Cross product of lists using heterogenous lists. *)
-  Definition Join_Lists
-             {A : Type}
-             {f : A -> Type}
-             {As : list A}
-             {a : A}
-             (l' : list (ilist f As))
-             (c : ilist f As -> Comp (list (f a)))
-  : Comp (list (ilist f (a :: As))) :=
-    flatten_CompList (map (fun l' => l <- c l'; ret (map (fun fa => icons _ fa l') l)) l').
-
-  Definition Build_single_Tuple_list
-             {heading}
-             (l : list (@Tuple heading))
-  : list (ilist (@Tuple) [heading])
-    := map (fun a => icons _ a (inil _)) l.
-
-  Lemma filter_and_join_ilist_tail
-        {A}
-        {a}
-        {As}
-        (f' : A -> Type)
-  : forall
-      (f : (ilist f' As) -> bool)
-      (s1 : list (ilist f' As))
-      (s2 : ilist f' As -> Comp (list (f' a)))
-      filter_rest,
-      (forall a, List.In a s1 -> exists v, computes_to (s2 a) v)
-      -> refineEquiv (l <- (Join_Lists s1 s2);
-                   ret (filter (fun x : ilist f' (a :: As) => f (ilist_tl x) && filter_rest x) l))
-                     (l <- Join_Lists (filter f s1) s2;
-                      ret (filter filter_rest l)).
-  Proof.
-    split; induction s1; unfold Join_Lists in *; simpl in *; intros; eauto.
-    - simplify with monad laws; simpl; intros v Comp_v;
-      inversion_by computes_to_inv; subst; repeat econstructor.
-    - simplify with monad laws; intros v.
-      case_eq (f a0); simpl; intros a0_eq Comp_v.
-      + inversion_by computes_to_inv; subst; econstructor; eauto.
-        pose (IHs1 (fun a In_a => H _ (or_intror In_a)) _ (BindComputes _ H3 (ReturnComputes _))); inversion_by computes_to_inv; subst.
-        econstructor; eauto.
-        repeat rewrite filter_app, filter_map; rewrite H4; simpl.
-        rewrite a0_eq, filter_and, filter_true; eauto.
-      + pose (IHs1 (fun a In_a => H _ (or_intror In_a)) _ Comp_v); inversion_by computes_to_inv; subst.
-        destruct (H a0); eauto.
-        repeat (econstructor; eauto).
-        rewrite filter_app, filter_map; simpl; intros;
-        rewrite a0_eq, filter_false; constructor.
-    - intros v Comp_v; inversion_by computes_to_inv; subst; eauto.
-    - intros v Comp_v; inversion_by computes_to_inv; subst.
-      pose proof (IHs1 (fun a In_a => H _ (or_intror In_a)) _
-                 (BindComputes _ H3 (ReturnComputes _))).
-      inversion_by computes_to_inv.
-      case_eq (f a0); intros a0_eq; simpl.
-      + repeat (econstructor; eauto).
-        repeat rewrite filter_app, filter_map; rewrite H4, filter_and; simpl.
-        rewrite a0_eq, filter_and, filter_true; eauto.
-      + repeat (econstructor; eauto).
-        repeat rewrite filter_app, filter_map, filter_and; rewrite H4; simpl.
-        rewrite a0_eq, filter_false; eauto.
-  Qed.
-
-  Corollary filter_join_ilist_tail
-        {A}
-        {a}
-        {As}
-        (f' : A -> Type)
-  : forall
-      (f : (ilist f' As) -> bool)
-      (s1 : list (ilist f' As))
-      (s2 : ilist f' As -> Comp (list (f' a))),
-      (forall a, List.In a s1 -> exists v, computes_to (s2 a) v)
-      -> refineEquiv (l <- (Join_Lists s1 s2);
-                   ret (filter (fun x : ilist f' (a :: As) => f (ilist_tl x)) l))
-                     (Join_Lists (filter f s1) s2).
-  Proof.
-    intros; pose proof (filter_and_join_ilist_tail f s1 s2 (fun _ => true)).
-    setoid_rewrite filter_and in H0; setoid_rewrite filter_true in H0.
-    setoid_rewrite H0; eauto; setoid_rewrite refineEquiv_unit_bind; reflexivity.
   Qed.
 
   Lemma refine_Query_In_Enumerate
@@ -168,9 +87,11 @@ Section BagsQueryStructureRefinements.
       -> forall (idx : BoundedString)
                 (resultComp : Tuple -> Comp (list ResultT)),
            refine (UnConstrQuery_In r_o idx resultComp)
-                  (l <- CallBagMethod idx {|bindex := "Enumerate" |} r_n ();
-                   List_Query_In (Build_single_Tuple_list (snd l))
-                                 (fun tup => resultComp (ilist_hd tup))) .
+                  (l <- Join_Comp_Lists [ inil _ ]
+                     (fun _ =>
+                        l <- CallBagMethod idx {|bindex := "Enumerate" |} r_n ();
+                      (ret (snd l)));
+                   (List_Query_In l (fun tup : ilist (@Tuple) [ _ ]=> resultComp (ilist_hd tup)))) .
   Proof.
     unfold UnConstrQuery_In, QueryResultComp, CallBagMethod;
     intros; simpl.
@@ -183,8 +104,10 @@ Section BagsQueryStructureRefinements.
     intuition; destruct_ex; intuition; subst.
     econstructor; eauto.
     econstructor; rewrite ((proj1 H) idx); eauto.
-    unfold Build_single_Tuple_list in *; rewrite map_map.
-    repeat rewrite map_map in H2; simpl in *; eauto.
+    rewrite map_map.
+    repeat setoid_rewrite map_app in H3;
+      repeat setoid_rewrite map_map in H3; simpl in *;
+      rewrite app_nil_r in H3; eauto.
   Qed.
 
   Local Transparent Query_For.
@@ -207,24 +130,6 @@ Section BagsQueryStructureRefinements.
     subst; econstructor; econstructor; eauto.
   Qed.
 
-  Lemma flatten_CompList_app_inv
-        {A : Type}
-  : forall (l l' : list (Comp (list A))) v,
-      flatten_CompList (l ++ l') ↝ v
-      -> exists e e',
-           v = app e e'
-           /\ flatten_CompList l ↝ e
-           /\ flatten_CompList l' ↝ e'.
-  Proof.
-    induction l; simpl; intros.
-    - eexists []; exists v; simpl; intuition.
-    - inversion_by computes_to_inv; subst.
-      destruct (IHl _ _ H1) as [e [e' [v_eq [Comp_l Comp_l']]]].
-      rewrite v_eq.
-      exists (app x e); exists e'; intuition.
-      repeat econstructor; eauto.
-  Qed.
-
   Lemma refine_Join_Query_In_Enumerate'
         headings
         (ResultT : Type) :
@@ -237,12 +142,12 @@ Section BagsQueryStructureRefinements.
              l,
         refine (List_Query_In l (fun tup : ilist (@Tuple) headings =>
                                    UnConstrQuery_In r_o idx (resultComp tup)))
-               (l' <- (Join_Lists l (fun _ => l <- (CallBagMethod idx {|bindex := "Enumerate" |} r_n ());
-                                     ret (snd l)));
+               (l' <- (Join_Comp_Lists l (fun _ => l <- (CallBagMethod idx {|bindex := "Enumerate" |} r_n ());
+                                          ret (snd l)));
                 List_Query_In l' (fun tup_pair => (resultComp (ilist_tl tup_pair) (ilist_hd tup_pair)))).
   Proof.
     intros.
-    unfold List_Query_In; induction l; unfold Join_Lists; simpl.
+    unfold List_Query_In; induction l; unfold Join_Comp_Lists; simpl.
     - intros v Comp_v; inversion_by computes_to_inv; subst; eauto.
     - setoid_rewrite IHl; rewrite refine_Query_In_Enumerate; eauto.
       unfold List_Query_In.
@@ -252,14 +157,14 @@ Section BagsQueryStructureRefinements.
       subst.
       rewrite map_app, map_map in H2; simpl in *.
       econstructor; eauto.
-      apply flatten_CompList_app_inv in H2; destruct_ex; intuition.
+      apply flatten_CompList_app_inv' in H2; destruct_ex; intuition.
       subst; repeat (econstructor; eauto).
-      unfold Build_single_Tuple_list in *; rewrite map_map; simpl;
-      eauto.
+      unfold Build_single_Tuple_list in *.
+      rewrite !map_app, !map_map, app_nil_r; simpl; eauto.
   Qed.
 
   Corollary refine_Join_Query_In_Enumerate
-        (ResultT : Type) :
+            (ResultT : Type) :
     forall r_o (r_n : IndexedQueryStructure qs_schema BagIndexKeys),
       DelegateToBag_AbsR r_o r_n ->
       forall (idx idx' : BoundedString)
@@ -269,9 +174,9 @@ Section BagsQueryStructureRefinements.
                               (fun tup =>
                                  UnConstrQuery_In r_o idx' (resultComp (ilist_hd tup))))
                (l <- CallBagMethod idx {|bindex := "Enumerate" |} r_n ();
-                l' <- (Join_Lists (Build_single_Tuple_list (snd l))
-                                  (fun _ => l <- (CallBagMethod idx' {|bindex := "Enumerate" |} r_n ());
-                                   ret (snd l)));
+                l' <- (Join_Comp_Lists (Build_single_Tuple_list (snd l))
+                                       (fun _ => l <- (CallBagMethod idx' {|bindex := "Enumerate" |} r_n ());
+                                        ret (snd l)));
                 List_Query_In l' (fun tup_pair => (resultComp (ilist_hd (ilist_tl tup_pair)) (ilist_hd tup_pair)))).
   Proof.
     intros.
@@ -280,20 +185,39 @@ Section BagsQueryStructureRefinements.
   Qed.
 
   Lemma refine_Join_Enumerate_Swap
+        (ResultT : Type) :
+    forall r_o (r_n : IndexedQueryStructure qs_schema BagIndexKeys),
+      DelegateToBag_AbsR r_o r_n ->
+      forall (idx idx' : BoundedString)
+             (resultComp : _ -> Comp (list ResultT)),
+        refine (l <- CallBagMethod idx {|bindex := "Enumerate" |} r_n ();
+                l' <- (Join_Comp_Lists (Build_single_Tuple_list (snd l))
+                                       (fun _ => l <- (CallBagMethod idx' {|bindex := "Enumerate" |} r_n ());
+                                        ret (snd l)));
+                List_Query_In l' resultComp)
+               (l <- CallBagMethod idx' {|bindex := "Enumerate" |} r_n ();
+                l' <- (Join_Comp_Lists (Build_single_Tuple_list (snd l))
+                                       (fun _ => l <- (CallBagMethod idx {|bindex := "Enumerate" |} r_n ());
+                                        ret (snd l)));
+                List_Query_In l' (fun tup_pair => (resultComp (icons _ (ilist_hd (ilist_tl tup_pair)) (icons _ (ilist_hd tup_pair) (inil _)))))).
+  Proof.
+  Admitted.
+
+  (* Lemma refine_Join_Enumerate_Swap
         (A B ResultT : Type) :
     forall (c : Comp A) (c' : Comp B)
            (resultComp : _ -> _ -> Comp (list ResultT)),
       refineEquiv (For (l <- c;
-                   l' <- c';
-                   resultComp l l'))
-                (For (l' <- c';
-                      l <- c;
-                      resultComp l l')).
+                        l' <- c';
+                        resultComp l l'))
+                  (For (l' <- c';
+                        l <- c;
+                        resultComp l l')).
   Proof.
     split; simpl; intros; f_equiv; intros v Comp_v;
     inversion_by computes_to_inv; subst;
     repeat (econstructor; eauto).
-  Qed.
+  Qed.*)
 
   Lemma refine_Query_For_In_Find
         (ResultT : Type)
@@ -321,6 +245,90 @@ Section BagsQueryStructureRefinements.
     reflexivity.
   Qed.
 
+  Lemma refine_Join_Comp_Lists_To_Find
+  : forall r_o (r_n : IndexedQueryStructure qs_schema BagIndexKeys),
+      DelegateToBag_AbsR r_o r_n
+      -> forall {headings}
+                (l1 : list (ilist (@Tuple) headings))
+                (idx : @BoundedString (map relName (qschemaSchemas qs_schema)))
+                search_pattern,
+           refine (Join_Filtered_Comp_Lists l1
+                                            (fun _ =>
+                                               l <- CallBagMethod idx {|bindex := "Enumerate" |} r_n ();
+                                             ret (snd l))
+                                            (fun a => BagMatchSearchTerm (ith_Bounded relName BagIndexKeys idx) search_pattern (ilist_hd a) && true))
+                  (Join_Comp_Lists l1
+                                   (fun _ =>
+                                      l <- CallBagMethod idx {|bindex := "Find" |} r_n search_pattern;
+                                    ret (snd l))) .
+  Proof.
+    unfold Join_Filtered_Comp_Lists, Join_Comp_Lists; intros; simpl.
+    induction l1.
+    - simplify with monad laws; reflexivity.
+    - Local Transparent CallBagMethod.
+      unfold CallBagMethod.
+      simpl.
+      setoid_rewrite refineEquiv_bind_bind.
+      setoid_rewrite refineEquiv_bind_bind.
+      setoid_rewrite refineEquiv_bind_bind.
+      setoid_rewrite refineEquiv_bind_bind at 1.
+      repeat setoid_rewrite refineEquiv_bind_unit; simpl;
+      f_equiv; intro.
+      setoid_rewrite refineEquiv_bind_bind at 1.
+      repeat setoid_rewrite refineEquiv_bind_unit; simpl.
+      intros v Comp_v.
+      inversion_by computes_to_inv; subst.
+      generalize (IHl1 _ H1); intros; inversion_by computes_to_inv.
+      econstructor; subst; eauto.
+      rewrite filter_app, filter_map.
+      simpl.
+      erewrite filter_by_equiv; eauto.
+      unfold ExtensionalEq; intros; rewrite andb_true_r; auto.
+  Qed.
+
+  Lemma refine_Join_Comp_Lists_To_Find_dep
+  : forall r_o (r_n : IndexedQueryStructure qs_schema BagIndexKeys),
+      DelegateToBag_AbsR r_o r_n
+      -> forall {headings}
+                (l1 : list (ilist (@Tuple) headings))
+                (idx : @BoundedString (map relName (qschemaSchemas qs_schema)))
+                (search_pattern : ilist (@Tuple) headings -> _),
+           refine (Join_Filtered_Comp_Lists l1
+                                            (fun _ =>
+                                               l <- CallBagMethod idx {|bindex := "Enumerate" |} r_n ();
+                                             ret (snd l))
+                                            (fun a => BagMatchSearchTerm (ith_Bounded relName BagIndexKeys idx)
+                                                                         (search_pattern (ilist_tl a)) (ilist_hd a) && true))
+                  (Join_Comp_Lists l1
+                                   (fun a =>
+                                      l <- CallBagMethod idx {|bindex := "Find" |} r_n (search_pattern a);
+                                    ret (snd l))) .
+  Proof.
+    unfold Join_Filtered_Comp_Lists, Join_Comp_Lists; intros; simpl.
+    induction l1.
+    - simplify with monad laws; reflexivity.
+    - Local Transparent CallBagMethod.
+      unfold CallBagMethod.
+      simpl.
+      setoid_rewrite refineEquiv_bind_bind.
+      setoid_rewrite refineEquiv_bind_bind.
+      setoid_rewrite refineEquiv_bind_bind.
+      setoid_rewrite refineEquiv_bind_bind at 1.
+      repeat setoid_rewrite refineEquiv_bind_unit; simpl;
+      f_equiv; intro.
+      setoid_rewrite refineEquiv_bind_bind at 1.
+      repeat setoid_rewrite refineEquiv_bind_unit; simpl.
+      intros v Comp_v.
+      inversion_by computes_to_inv; subst.
+      generalize (IHl1 _ H1); intros; inversion_by computes_to_inv.
+      econstructor; subst; eauto.
+      rewrite filter_app, filter_map.
+      simpl.
+      erewrite filter_by_equiv; eauto.
+      unfold ExtensionalEq; intros; rewrite andb_true_r; auto.
+  Qed.
+
+
   Instance DecideableEnsemblePair_tail
            {A}
            {a}
@@ -347,15 +355,15 @@ Section BagsQueryStructureRefinements.
     intro; apply (dec_decides_P (DecideableEnsemble := P_dec) (ilist_hd a0)).
   Defined.
 
-  Lemma Join_Lists_nil
+  Lemma Join_Comp_Lists_nil
         {A}
         {a}
         {As}
         (f' : A -> Type)
   : forall (s2 : _ -> Comp (list (f' a))),
-      refineEquiv (Join_Lists (As := As) (a := a) [] s2) (ret []).
+      refineEquiv (Join_Comp_Lists (As := As) (a := a) [] s2) (ret []).
   Proof.
-    unfold Join_Lists; simpl; try reflexivity.
+    unfold Join_Comp_Lists; simpl; try reflexivity.
   Qed.
 
   Lemma filter_and_join_ilist_hd
@@ -368,12 +376,12 @@ Section BagsQueryStructureRefinements.
       (s1 : list (ilist f' As))
       (s2 : _ -> Comp (list (f' a)))
       filter_rest ,
-      refineEquiv (l <- (Join_Lists s1 s2);
+      refineEquiv (l <- (Join_Comp_Lists s1 s2);
                    ret (filter (fun x : ilist f' (a :: As) => f (ilist_hd x) && filter_rest x) l))
-                  (l <- Join_Lists s1 (fun a => l <- s2 a; ret (filter f l));
+                  (l <- Join_Comp_Lists s1 (fun a => l <- s2 a; ret (filter f l));
                    ret (filter filter_rest l)).
   Proof.
-    split; induction s1; unfold Join_Lists in *; simpl in *; intros; eauto.
+    split; induction s1; unfold Join_Comp_Lists in *; simpl in *; intros; eauto.
     - simplify with monad laws; rewrite refineEquiv_bind_unit;
       reflexivity.
     - simplify with monad laws; intros v Comp_v;
@@ -394,18 +402,18 @@ Section BagsQueryStructureRefinements.
       rewrite <- filter_and, H3; eauto.
   Qed.
 
-    Corollary filter_join_ilist_hd
-        {A}
-        {a}
-        {As}
-        (f' : A -> Type)
+  Corollary filter_join_ilist_hd
+            {A}
+            {a}
+            {As}
+            (f' : A -> Type)
   : forall
       (f : f' a -> bool)
       (s1 : list (ilist f' As))
       (s2 : _ -> Comp (list (f' a))),
-      refineEquiv (l <- (Join_Lists s1 s2);
+      refineEquiv (l <- (Join_Comp_Lists s1 s2);
                    ret (filter (fun x : ilist f' (a :: As) => f (ilist_hd x)) l))
-                  (Join_Lists s1 (fun a => l <- s2 a; ret (filter f l))).
+                  (Join_Comp_Lists s1 (fun a => l <- s2 a; ret (filter f l))).
   Proof.
     intros; pose proof (filter_and_join_ilist_hd f s1 s2 (fun _ => true)).
     setoid_rewrite filter_and in H; setoid_rewrite filter_true in H.
@@ -423,7 +431,7 @@ Section BagsQueryStructureRefinements.
   Qed.
 
   Corollary refine_Query_For_In_Find_snd'
-        (ResultT : Type)
+            (ResultT : Type)
   : forall r_o (r_n : IndexedQueryStructure qs_schema BagIndexKeys),
       DelegateToBag_AbsR r_o r_n
       ->
@@ -434,15 +442,15 @@ Section BagsQueryStructureRefinements.
         ExtensionalEq filter_dec
                       (BagMatchSearchTerm (ith_Bounded relName BagIndexKeys idx) search_pattern)
         -> refine (l <- CallBagMethod idx {|bindex := "Enumerate" |} r_n ();
-                        List_Query_In (filter (fun tup : ilist (@Tuple) [_] => filter_dec (ilist_hd tup)) (Build_single_Tuple_list (snd l)))
-                                      resultComp)
+                   List_Query_In (filter (fun tup : ilist (@Tuple) [_] => filter_dec (ilist_hd tup)) (Build_single_Tuple_list (snd l)))
+                                 resultComp)
                   (l <- CallBagMethod idx {|bindex := "Find" |} r_n search_pattern;
                    List_Query_In (Build_single_Tuple_list (snd l)) resultComp).
   Proof.
     simpl; intros.
     setoid_rewrite filter_Build_single_Tuple_list.
     unfold UnConstrQuery_In, QueryResultComp, CallBagMethod, Query_For;
-    intros; simpl.
+      intros; simpl.
     simplify with monad laws.
     setoid_rewrite refineEquiv_bind_bind;
       setoid_rewrite refineEquiv_bind_unit; simpl; f_equiv; intro.
@@ -451,28 +459,28 @@ Section BagsQueryStructureRefinements.
     reflexivity.
   Qed.
 
-    Corollary refine_Query_For_In_Find_single
-              (ResultT : Type)
-    : forall r_o (r_n : IndexedQueryStructure qs_schema BagIndexKeys),
-        DelegateToBag_AbsR r_o r_n ->
+  Corollary refine_Query_For_In_Find_single
+            (ResultT : Type)
+  : forall r_o (r_n : IndexedQueryStructure qs_schema BagIndexKeys),
+      DelegateToBag_AbsR r_o r_n ->
       forall (idx : @BoundedString (map relName (qschemaSchemas qs_schema)))
              search_pattern
              (resultComp : _ -> Comp (list ResultT))
              filter_rest,
         refine (l <- CallBagMethod idx {|bindex := "Enumerate" |} r_n ();
-                   List_Query_In (filter (fun a : ilist (@Tuple) [_] => BagMatchSearchTerm _ search_pattern (ilist_hd a) && filter_rest a) (Build_single_Tuple_list (snd l)))
-                                 resultComp)
-                  (l <- CallBagMethod idx {|bindex := "Find" |} r_n search_pattern;
-                   List_Query_In (filter filter_rest (Build_single_Tuple_list (snd l))) resultComp).
-    Proof.
-      unfold CallBagMethod; simpl; intros.
-      simplify with monad laws.
-      setoid_rewrite refineEquiv_bind_bind;
-        setoid_rewrite refineEquiv_bind_unit; simpl;
-        f_equiv; intro.
-      setoid_rewrite <- filter_Build_single_Tuple_list; rewrite filter_and;
-      f_equiv.
-    Qed.
+                List_Query_In (filter (fun a : ilist (@Tuple) [_] => BagMatchSearchTerm _ search_pattern (ilist_hd a) && filter_rest a) (Build_single_Tuple_list (snd l)))
+                              resultComp)
+               (l <- CallBagMethod idx {|bindex := "Find" |} r_n search_pattern;
+                List_Query_In (filter filter_rest (Build_single_Tuple_list (snd l))) resultComp).
+  Proof.
+    unfold CallBagMethod; simpl; intros.
+    simplify with monad laws.
+    setoid_rewrite refineEquiv_bind_bind;
+      setoid_rewrite refineEquiv_bind_unit; simpl;
+      f_equiv; intro.
+    setoid_rewrite <- filter_Build_single_Tuple_list; rewrite filter_and;
+    f_equiv.
+  Qed.
 
   Add Parametric Morphism
       (A : Type)
@@ -480,18 +488,18 @@ Section BagsQueryStructureRefinements.
       (As : list A)
       (a : A)
       (l' : list (ilist f As))
-      : (@Join_Lists A f As a l')
+  : (@Join_Comp_Lists A f As a l')
       with signature
       (pointwise_relation _ refineEquiv) ==> refineEquiv
-        as refineEquiv_Join_Lists.
+        as refineEquiv_Join_Comp_Lists.
   Proof.
     unfold pointwise_relation; simpl; intros.
-    induction l'; unfold Join_Lists; simpl.
+    induction l'; unfold Join_Comp_Lists; simpl.
     - reflexivity.
     - rewrite H; setoid_rewrite IHl'; reflexivity.
   Qed.
 
-  Lemma Join_Lists_apply_f
+  Lemma Join_Comp_Lists_apply_f
         {A B C : Type}
         {f : A -> Type}
   : forall (As : list A)
@@ -499,9 +507,9 @@ Section BagsQueryStructureRefinements.
            (l : list (ilist f As))
            (c : ilist f As -> Comp (list (f a)))
            (c' : B -> Comp C) (f' : list (ilist f (a :: As)) -> B),
-      refineEquiv (l' <- Join_Lists l c;
+      refineEquiv (l' <- Join_Comp_Lists l c;
                    c' (f' l'))
-                  (l' <- (l' <- Join_Lists l c; ret (f' l'));
+                  (l' <- (l' <- Join_Comp_Lists l c; ret (f' l'));
                    c' l').
   Proof.
     split; rewrite refineEquiv_bind_bind;
@@ -510,7 +518,7 @@ Section BagsQueryStructureRefinements.
     try econstructor; eauto.
   Qed.
 
-  Lemma refine_Join_Lists_filter_search_term_snd
+  Lemma refine_Join_Comp_Lists_filter_search_term_snd
         (ResultT : Type) :
     forall (r_n : IndexedQueryStructure qs_schema BagIndexKeys)
            headings
@@ -519,20 +527,20 @@ Section BagsQueryStructureRefinements.
            (resultComp : ilist (@Tuple) (_ :: headings) -> Comp (list ResultT))
            filter_rest
            cl,
-      refine (l' <- (Join_Lists cl
-                          (fun _ => l <- CallBagMethod idx' {| bindex := "Enumerate" |} r_n ();
-                           ret (snd l)));
-                 List_Query_In (filter (fun a : ilist (@Tuple) (_ :: headings) => BagMatchSearchTerm _ search_pattern (ilist_hd a) && filter_rest a) l')
-                               resultComp)
-                (l' <- (Join_Lists cl
-                                   (fun _ => l <- CallBagMethod idx' {| bindex := "Find" |} r_n search_pattern;
-                                             ret (snd l)));
-                      List_Query_In (filter filter_rest l') resultComp).
+      refine (l' <- (Join_Comp_Lists cl
+                                     (fun _ => l <- CallBagMethod idx' {| bindex := "Enumerate" |} r_n ();
+                                      ret (snd l)));
+              List_Query_In (filter (fun a : ilist (@Tuple) (_ :: headings) => BagMatchSearchTerm _ search_pattern (ilist_hd a) && filter_rest a) l')
+                            resultComp)
+             (l' <- (Join_Comp_Lists cl
+                                     (fun _ => l <- CallBagMethod idx' {| bindex := "Find" |} r_n search_pattern;
+                                      ret (snd l)));
+              List_Query_In (filter filter_rest l') resultComp).
   Proof.
     intros; unfold CallBagMethod; simpl.
     repeat setoid_rewrite (refineEquiv_bind_bind);
       repeat setoid_rewrite refineEquiv_bind_unit; simpl.
-    setoid_rewrite Join_Lists_apply_f
+    setoid_rewrite Join_Comp_Lists_apply_f
     with (c' := fun l =>  List_Query_In l _).
     setoid_rewrite (refineEquiv_bind_bind) at 2;
       repeat setoid_rewrite refineEquiv_bind_unit; simpl.
@@ -547,27 +555,27 @@ Section BagsQueryStructureRefinements.
     simplify with monad laws; f_equiv.
   Qed.
 
-  Corollary refine_Join_Lists_filter_search_term_snd'
-        (ResultT : Type) :
+  Corollary refine_Join_Comp_Lists_filter_search_term_snd'
+            (ResultT : Type) :
     forall (r_n : IndexedQueryStructure qs_schema BagIndexKeys)
            idx idx'
            search_pattern
            (resultComp : ilist (@Tuple) [_; _] -> Comp (list ResultT))
            filter_rest,
       refine (cl <- CallBagMethod idx {| bindex := "Enumerate" |} r_n ();
-              l' <- (Join_Lists (Build_single_Tuple_list (snd cl))
-                          (fun _ => l <- CallBagMethod idx' {| bindex := "Enumerate" |} r_n ();
-                           ret (snd l)));
-                 List_Query_In (filter (fun a : ilist (@Tuple) [_ ; _] => BagMatchSearchTerm _ search_pattern (ilist_hd a) && filter_rest a) l')
-                               resultComp)
+              l' <- (Join_Comp_Lists (Build_single_Tuple_list (snd cl))
+                                     (fun _ => l <- CallBagMethod idx' {| bindex := "Enumerate" |} r_n ();
+                                      ret (snd l)));
+              List_Query_In (filter (fun a : ilist (@Tuple) [_ ; _] => BagMatchSearchTerm _ search_pattern (ilist_hd a) && filter_rest a) l')
+                            resultComp)
              (cl <- CallBagMethod idx {| bindex := "Enumerate" |} r_n ();
-              l' <- (Join_Lists (Build_single_Tuple_list (snd cl))
-                                   (fun _ => l <- CallBagMethod idx' {| bindex := "Find" |} r_n search_pattern;
-                                             ret (snd l)));
-                      List_Query_In (filter filter_rest l') resultComp).
+              l' <- (Join_Comp_Lists (Build_single_Tuple_list (snd cl))
+                                     (fun _ => l <- CallBagMethod idx' {| bindex := "Find" |} r_n search_pattern;
+                                      ret (snd l)));
+              List_Query_In (filter filter_rest l') resultComp).
   Proof.
     intros; f_equiv; intro.
-    apply refine_Join_Lists_filter_search_term_snd.
+    apply refine_Join_Comp_Lists_filter_search_term_snd.
   Qed.
 
   Lemma refine_List_Query_In_Return
@@ -593,12 +601,12 @@ Section BagsQueryStructureRefinements.
       (s1 : list (ilist f' As))
       (s2 : _ -> Comp (list (f' a)))
       filter_rest,
-      refineEquiv (l <- (Join_Lists s1 s2);
+      refineEquiv (l <- (Join_Comp_Lists s1 s2);
                    ret (filter (fun x : ilist f' (a :: As) => f (ilist_tl x) (ilist_hd x) && filter_rest x) l))
-                  (l <- Join_Lists s1 (fun a => l <- s2 a; ret (filter (f a) l));
+                  (l <- Join_Comp_Lists s1 (fun a => l <- s2 a; ret (filter (f a) l));
                    ret (filter filter_rest l)).
   Proof.
-    split; induction s1; unfold Join_Lists in *; simpl in *; intros; eauto.
+    split; induction s1; unfold Join_Comp_Lists in *; simpl in *; intros; eauto.
     - simplify with monad laws; rewrite refineEquiv_bind_unit; reflexivity.
     - simplify with monad laws; intros v Comp_v;
       inversion_by computes_to_inv; subst; econstructor; eauto.
@@ -618,7 +626,7 @@ Section BagsQueryStructureRefinements.
       rewrite <- filter_and, H3; eauto.
   Qed.
 
-    Lemma refine_Join_Lists_filter_search_term_snd_dep
+  Lemma refine_Join_Comp_Lists_filter_search_term_snd_dep
         (ResultT : Type) :
     forall (r_n : IndexedQueryStructure qs_schema BagIndexKeys)
            headings
@@ -627,31 +635,31 @@ Section BagsQueryStructureRefinements.
            (resultComp : ilist (@Tuple) (_ :: headings) -> Comp (list ResultT))
            filter_rest
            (cl : list (ilist (@Tuple) headings)),
-      refine (l' <- (Join_Lists cl
-                          (fun _ => l <- CallBagMethod idx' {| bindex := "Enumerate" |} r_n ();
-                           ret (snd l)));
-                 List_Query_In (filter (fun a : ilist (@Tuple) (_ :: headings) => BagMatchSearchTerm _ (search_pattern (ilist_tl a)) (ilist_hd a) && filter_rest a) l')
-                               resultComp)
-                (l' <- (Join_Lists cl
-                                   (fun tup => l <- CallBagMethod idx' {| bindex := "Find" |} r_n (search_pattern tup);
-                                             ret (snd l)));
-                      List_Query_In (filter filter_rest l') resultComp).
+      refine (l' <- (Join_Comp_Lists cl
+                                     (fun _ => l <- CallBagMethod idx' {| bindex := "Enumerate" |} r_n ();
+                                      ret (snd l)));
+              List_Query_In (filter (fun a : ilist (@Tuple) (_ :: headings) => BagMatchSearchTerm _ (search_pattern (ilist_tl a)) (ilist_hd a) && filter_rest a) l')
+                            resultComp)
+             (l' <- (Join_Comp_Lists cl
+                                     (fun tup => l <- CallBagMethod idx' {| bindex := "Find" |} r_n (search_pattern tup);
+                                      ret (snd l)));
+              List_Query_In (filter filter_rest l') resultComp).
   Proof.
     intros; unfold CallBagMethod; simpl.
     repeat setoid_rewrite (refineEquiv_bind_bind);
       repeat setoid_rewrite refineEquiv_bind_unit; simpl.
-    setoid_rewrite Join_Lists_apply_f
+    setoid_rewrite Join_Comp_Lists_apply_f
     with (c' := fun l =>  List_Query_In l _).
     setoid_rewrite (refineEquiv_bind_bind) at 2;
       repeat setoid_rewrite refineEquiv_bind_unit; simpl.
     setoid_rewrite refineEquiv_unit_bind; simpl.
     rewrite filter_and_join_ilist_hd_dep with
     (f := fun tup =>  (BagMatchSearchTerm
-                (ith_Bounded' relName (qschemaSchemas qs_schema)
-                   (nth_error_map relName (ibound idx')
-                      (qschemaSchemas qs_schema) (boundi idx'))
-                   (ith_error BagIndexKeys (ibound idx')))
-                (search_pattern tup))).
+                         (ith_Bounded' relName (qschemaSchemas qs_schema)
+                                       (nth_error_map relName (ibound idx')
+                                                      (qschemaSchemas qs_schema) (boundi idx'))
+                                       (ith_error BagIndexKeys (ibound idx')))
+                         (search_pattern tup))).
     simplify with monad laws; f_equiv.
   Qed.
 
@@ -662,12 +670,16 @@ Section BagsQueryStructureRefinements.
       idx,
       DelegateToBag_AbsR r_o r_n ->
       exists v : list Tuple,
-        (l <- CallBagMethod idx {| bindex := "Enumerate"|} r_n ();
-         ret (snd l)) ↝ v.
+        refine
+          (l <- CallBagMethod idx {| bindex := "Enumerate"|} r_n ();
+           ret (snd l))
+          (ret v).
   Proof.
     intros; destruct H as [r_o_eq H]; destruct (H idx) as [l l_eqv].
     rewrite (r_o_eq idx) in l_eqv.
-    eexists l; unfold CallBagMethod; simpl; eauto.
+    Local Transparent CallBagMethod.
+    eexists l; unfold CallBagMethod; simpl; simplify with monad laws.
+    econstructor; inversion_by computes_to_inv; subst; eauto.
   Qed.
 
   Lemma realizeable_Find
@@ -677,40 +689,40 @@ Section BagsQueryStructureRefinements.
       idx st,
       DelegateToBag_AbsR r_o r_n ->
       exists v : list Tuple,
-        (l <- CallBagMethod idx {| bindex := "Find"|} r_n st;
-         ret (snd l)) ↝ v.
+        refine (l <- CallBagMethod idx {| bindex := "Find"|} r_n st;
+                ret (snd l))
+               (ret v).
   Proof.
     intros; destruct H as [r_o_eq H]; destruct (H idx) as [l l_eqv].
     rewrite (r_o_eq idx) in l_eqv.
     eexists (filter _ l); unfold CallBagMethod; simpl; eauto.
     econstructor; eauto.
-    simpl; eauto.
   Qed.
 
-  Corollary refine_Join_Lists_filter_search_term_snd_dep'
-        (ResultT : Type) :
+  Corollary refine_Join_Comp_Lists_filter_search_term_snd_dep'
+            (ResultT : Type) :
     forall (r_n : IndexedQueryStructure qs_schema BagIndexKeys)
            idx idx'
            (search_pattern : _ -> _)
            (resultComp : ilist (@Tuple) [_; _] -> Comp (list ResultT))
            filter_rest,
       refine (cl <- CallBagMethod idx {| bindex := "Enumerate" |} r_n ();
-              l' <- (Join_Lists (Build_single_Tuple_list (snd cl))
-                          (fun _ => l <- CallBagMethod idx' {| bindex := "Enumerate" |} r_n ();
-                           ret (snd l)));
-                 List_Query_In (filter (fun a : ilist (@Tuple) [_ ; _] => BagMatchSearchTerm _ (search_pattern (ilist_tl a)) (ilist_hd a) && filter_rest a) l')
-                               resultComp)
+              l' <- (Join_Comp_Lists (Build_single_Tuple_list (snd cl))
+                                     (fun _ => l <- CallBagMethod idx' {| bindex := "Enumerate" |} r_n ();
+                                      ret (snd l)));
+              List_Query_In (filter (fun a : ilist (@Tuple) [_ ; _] => BagMatchSearchTerm _ (search_pattern (ilist_tl a)) (ilist_hd a) && filter_rest a) l')
+                            resultComp)
              (cl <- CallBagMethod idx {| bindex := "Enumerate" |} r_n ();
-              l' <- (Join_Lists (Build_single_Tuple_list (snd cl))
-                                   (fun tup => l <- CallBagMethod idx' {| bindex := "Find" |} r_n (search_pattern tup);
-                                             ret (snd l)));
-                      List_Query_In (filter filter_rest l') resultComp).
+              l' <- (Join_Comp_Lists (Build_single_Tuple_list (snd cl))
+                                     (fun tup => l <- CallBagMethod idx' {| bindex := "Find" |} r_n (search_pattern tup);
+                                      ret (snd l)));
+              List_Query_In (filter filter_rest l') resultComp).
   Proof.
     intros; f_equiv; intro;
-    apply refine_Join_Lists_filter_search_term_snd_dep.
+    apply refine_Join_Comp_Lists_filter_search_term_snd_dep.
   Qed.
 
-  Lemma refine_Join_Lists_filter_search_term_fst
+  Lemma refine_Join_Comp_Lists_filter_search_term_fst
         (ResultT : Type) :
     forall (r_n : IndexedQueryStructure qs_schema BagIndexKeys)
            idx
@@ -721,24 +733,24 @@ Section BagsQueryStructureRefinements.
            (cl_realizable : forall a, exists v, computes_to (cl a) v)
            filter_rest,
       refine (l <- CallBagMethod idx {| bindex := "Enumerate" |} r_n ();
-              l' <- Join_Lists (Build_single_Tuple_list (snd l)) cl;
+              l' <- Join_Comp_Lists (Build_single_Tuple_list (snd l)) cl;
               List_Query_In (filter (fun a : ilist (@Tuple) [_ ; _] => (BagMatchSearchTerm _ search_pattern (ilist_hd (ilist_tl a)) && filter_rest a)) l')
                             resultComp)
              (l <- CallBagMethod idx {| bindex := "Find" |} r_n search_pattern;
-              l' <- Join_Lists (Build_single_Tuple_list (snd l)) cl;
+              l' <- Join_Comp_Lists (Build_single_Tuple_list (snd l)) cl;
               List_Query_In (filter filter_rest l') resultComp).
   Proof.
     intros; unfold CallBagMethod; simpl.
     repeat setoid_rewrite (refineEquiv_bind_bind);
       repeat setoid_rewrite refineEquiv_bind_unit; simpl.
     f_equiv; unfold pointwise_relation; intros.
-    setoid_rewrite Join_Lists_apply_f
+    setoid_rewrite Join_Comp_Lists_apply_f
     with (c' := fun l =>  List_Query_In l resultComp).
     setoid_rewrite (refineEquiv_bind_bind) at 2;
       repeat setoid_rewrite refineEquiv_bind_unit; simpl.
     rewrite (filter_and_join_ilist_tail
-              (fun a0 : ilist (@Tuple) [_] =>_ (ilist_hd a0))
-              (Build_single_Tuple_list a)) by eauto.
+               (fun a0 : ilist (@Tuple) [_] =>_ (ilist_hd a0))
+               (Build_single_Tuple_list a)) by eauto.
     simplify with monad laws; f_equiv.
     unfold Build_single_Tuple_list; simpl;
     repeat rewrite filter_map; f_equiv.
@@ -746,6 +758,22 @@ Section BagsQueryStructureRefinements.
 
 
   Require Import ADTSynthesis.QueryStructure.Implementation.Operations.General.DeleteRefinements.
+
+  Lemma refineEquiv_Join_Comp_Lists_Build_single_Tuple_list
+  : forall (r_n : IndexedQueryStructure qs_schema BagIndexKeys) idx,
+      refineEquiv (Join_Comp_Lists [inil (@Tuple)]
+                                   (fun _ : ilist (@Tuple) [] =>
+                                      l <- CallBagMethod idx ``("Enumerate") r_n ();
+                                    ret (snd l)))
+                  (l <- CallBagMethod idx ``("Enumerate") r_n ();
+                   ret (Build_single_Tuple_list (snd l))) .
+  Proof.
+    unfold Join_Comp_Lists, Build_single_Tuple_list; simpl; intros;
+    repeat setoid_rewrite refineEquiv_bind_bind;
+    repeat setoid_rewrite refineEquiv_bind_unit; f_equiv.
+    intros u.
+    rewrite app_nil_r; reflexivity.
+  Qed.
 
   Lemma refine_BagADT_QSDelete_fst :
     forall r_o (r_n : IndexedQueryStructure qs_schema BagIndexKeys),
@@ -766,7 +794,12 @@ Section BagsQueryStructureRefinements.
     setoid_rewrite refine_List_Query_In_Where.
     instantiate (1 := _).
     simpl in *.
-    setoid_rewrite (refine_Query_For_In_Find_snd' H _ H0).
+    rewrite (refineEquiv_Join_Comp_Lists_Build_single_Tuple_list r_n idx).
+    setoid_rewrite refineEquiv_bind_bind at 1.
+    setoid_rewrite refineEquiv_bind_bind at 1.
+    setoid_rewrite refineEquiv_bind_unit at 1.
+    setoid_rewrite <- refineEquiv_bind_bind at 1.
+    rewrite (refine_Query_For_In_Find_snd' H _ H0).
     setoid_rewrite refine_List_Query_In_Return.
     unfold Build_single_Tuple_list; setoid_rewrite map_map; simpl.
     setoid_rewrite map_id.
@@ -842,8 +875,8 @@ Section BagsQueryStructureRefinements.
         f_equal; eauto.
         * eapply H.
         * apply Extensionality_Ensembles. unfold Same_set, Included, In;
-          intuition; rewrite <- H0 in *;
-          eapply dec_decides_P; eauto.
+            intuition; rewrite <- H0 in *;
+            eapply dec_decides_P; eauto.
       + unfold GetUnConstrRelation, UpdateUnConstrRelation;
         rewrite ith_replace_BoundIndex_neq by eauto using string_dec.
         unfold GetIndexedRelation, UpdateIndexedRelation;
@@ -865,9 +898,9 @@ Section BagsQueryStructureRefinements.
           inversion H3; subst; rewrite (proj2 (Decides_false _ _)); eauto.
           rewrite filter_In in H3; intuition; constructor;
           [ apply l_eqv; eauto
-            | case_eq (dec (indexedElement x)); intros H'; rewrite H' in H5;
-              try discriminate;
-              eapply Decides_false in H'; eauto ].
+          | case_eq (dec (indexedElement x)); intros H'; rewrite H' in H5;
+            try discriminate;
+            eapply Decides_false in H'; eauto ].
           eapply NoDup_filter_map with (f := fun a => negb (dec a)); eauto.
       + rewrite get_update_unconstr_neq; eauto.
   Qed.
@@ -877,16 +910,16 @@ Section BagsQueryStructureRefinements.
       DelegateToBag_AbsR r_o r_n
       -> forall (idx : @BoundedString (map relName (qschemaSchemas qs_schema)))
                 t,
-          refine
-            (u <- { freshIdx | UnConstrFreshIdx (GetUnConstrRelation r_o idx) freshIdx };
-             {r_n' |
-              DelegateToBag_AbsR
-                (UpdateUnConstrRelation r_o idx (
-                                          EnsembleInsert
-                                            {| indexedElement := t; elementIndex := u |}
-                                            (GetUnConstrRelation r_o idx))) r_n'})
-            (l <- (CallBagMethod idx {|bindex := "Insert" |} r_n t);
-             ret (UpdateIndexedRelation r_n idx (fst l))).
+           refine
+             (u <- { freshIdx | UnConstrFreshIdx (GetUnConstrRelation r_o idx) freshIdx };
+              {r_n' |
+               DelegateToBag_AbsR
+                 (UpdateUnConstrRelation r_o idx (
+                                           EnsembleInsert
+                                             {| indexedElement := t; elementIndex := u |}
+                                             (GetUnConstrRelation r_o idx))) r_n'})
+             (l <- (CallBagMethod idx {|bindex := "Insert" |} r_n t);
+              ret (UpdateIndexedRelation r_n idx (fst l))).
   Proof.
     intros; unfold CallBagMethod, DelegateToBag_AbsR; simpl; destruct H as [H H'].
     repeat setoid_rewrite (refineEquiv_bind_bind);
@@ -894,9 +927,9 @@ Section BagsQueryStructureRefinements.
     rewrite H.
     apply refine_bind_pick; intros.
     unfold GetUnConstrRelation, UpdateUnConstrRelation in *;
-    unfold GetIndexedRelation, UpdateIndexedRelation in *;
-    refine pick val _; try reflexivity; try split;
-    intros; destruct (BoundedString_eq_dec idx idx0); subst.
+      unfold GetIndexedRelation, UpdateIndexedRelation in *;
+      refine pick val _; try reflexivity; try split;
+      intros; destruct (BoundedString_eq_dec idx idx0); subst.
     - rewrite ith_replace_BoundIndex_eq; rewrite i2th_replace_BoundIndex_eq.
       unfold Add, EnsembleInsert; apply Extensionality_Ensembles; split;
       unfold Included; intros; unfold In in *; destruct H1.
@@ -913,21 +946,21 @@ Section BagsQueryStructureRefinements.
                unfold EnsembleInsert in H1; destruct H1.
                * rewrite H1; simpl; omega.
                * apply H0 in H1; omega.
-      + unfold UnIndexedEnsembleListEquivalence;
-        exists ({| indexedElement := t; elementIndex := a |} :: l'); intuition.
-        * simpl; rewrite l'_eq; trivial.
-        * simpl; destruct H1;
-          [ left; symmetry; exact H1 | right; apply l_eqv; rewrite H; apply H1 ].
-        * unfold EnsembleInsert; destruct H1;
-          [ rewrite <- H1; left; trivial |
-          right; rewrite <- H; apply l_eqv in H1; unfold In in H1; exact H1 ].
-        * simpl; apply NoDup_cons;
-          [ unfold not; intros;
-            apply in_map_iff in H1; destruct H1; destruct H1;
-            apply l_eqv in H2; rewrite <- H in H0; unfold UnConstrFreshIdx in H0;
-              unfold In in H2; apply H0 in H2; omega | exact NoDup_l' ].
-    - rewrite ith_replace_BoundIndex_neq.
-      apply H'. apply string_dec. unfold not in *; intros; rewrite H1 in n; intuition.
+               + unfold UnIndexedEnsembleListEquivalence;
+                 exists ({| indexedElement := t; elementIndex := a |} :: l'); intuition.
+                 * simpl; rewrite l'_eq; trivial.
+                 * simpl; destruct H1;
+                   [ left; symmetry; exact H1 | right; apply l_eqv; rewrite H; apply H1 ].
+                 * unfold EnsembleInsert; destruct H1;
+                   [ rewrite <- H1; left; trivial |
+                     right; rewrite <- H; apply l_eqv in H1; unfold In in H1; exact H1 ].
+                 * simpl; apply NoDup_cons;
+                   [ unfold not; intros;
+                     apply in_map_iff in H1; destruct H1; destruct H1;
+                     apply l_eqv in H2; rewrite <- H in H0; unfold UnConstrFreshIdx in H0;
+                     unfold In in H2; apply H0 in H2; omega | exact NoDup_l' ].
+               - rewrite ith_replace_BoundIndex_neq.
+                 apply H'. apply string_dec. unfold not in *; intros; rewrite H1 in n; intuition.
   Qed.
 
 End BagsQueryStructureRefinements.
